StandardLibrary/src/CallMany.dfy
@@ -7,15 +7,20 @@ include "./UInt.dfy"
 /*
   Call a single function many times in many threads
 
-  CallMany(callee : Callee, innerIters : uint32, outerIters : uint32, threads : uint32)
+  CallMany(callee : Callee, serialIters : uint32, concurrentIters : uint32)
   This is effectively 
 
-  for i n 0..outerIters
-     for j in 0..innerIters
+  for i n 0..concurrentIters
+     for j in 0..serialIters
        callee(j, i)
 
-  but multi threaded.
-  Depending on the platform, the number of parallel threads is either `threads` or `outerIters`
+  but multi threaded, so really, in `concurrentIters` concurrent threads we execute
+
+     for j in 0..serialIters
+       callee(j, i)
+
+  The i and j passed to callee are generally useless, but can be helpful in certain types of debugging.
+
 */
 
 module {:extern "CallMany"} CallMany {
@@ -24,12 +29,16 @@ module {:extern "CallMany"} CallMany {
   import opened StandardLibrary.UInt
 
   trait {:termination false} Callee {
-    method call(inner : uint32, outer : uint32)
-      modifies (set o: object | true)
-    // modifies this, plus anything else that might be needed.
+    ghost var Modifies: set<object>
+    predicate ValidState() reads this
+
+    method call(serialPos : uint32, concurrentPos : uint32)
+      requires ValidState()
+      ensures ValidState()
+      modifies Modifies
   }
 
-  method {:extern "CallMany"} CallMany(callee : Callee, innerIters : uint32, outerIters : uint32, threads : uint32)
+  method {:extern "CallMany"} CallMany(callee : Callee, serialIters : uint32, concurrentIters : uint32)
 
 
 }
